backend/Unusedglobproof.v
@@ -1272,8 +1272,8 @@ Proof.
   assert (NO: gvar_volatile v = false).
   { unfold Genv.perm_globvar in H1. destruct (gvar_volatile v); auto. inv H1. }
 Local Transparent Mem.loadbytes.
-  generalize (S1 NO). unfold Mem.loadbytes. destruct Mem.range_perm_dec; destruct Mem.own_block_dec; intros E1; inv E1.
-  generalize (S2 NO). unfold Mem.loadbytes. destruct Mem.range_perm_dec; destruct Mem.own_block_dec; intros E2; inv E2.
+  generalize (S1 NO). unfold Mem.loadbytes. destruct Mem.range_perm_dec; destruct Mem.can_access_block_dec; intros E1; inv E1.
+  generalize (S2 NO). unfold Mem.loadbytes. destruct Mem.range_perm_dec; destruct Mem.can_access_block_dec; intros E2; inv E2.
   rewrite Z.add_0_r.
   apply Mem_getN_forall2 with (p := 0) (n := Z.to_nat (init_data_list_size (gvar_init v))).
   rewrite H3, H4. apply bytes_of_init_inject. auto.
