riscV/Asmgenproof1.v
@@ -1143,9 +1143,9 @@ Qed.
 Lemma indexed_load_access_correct:
   forall chunk (mk_instr: ireg -> offset -> instruction) rd m,
   (forall base ofs rs,
-     exec_instr ge fn (mk_instr base ofs) rs m = exec_load ge chunk rs m rd base ofs) ->
+     exec_instr ge fn (mk_instr base ofs) rs m (comp_of fn) = exec_load ge chunk rs m rd base ofs (comp_of fn) false) ->
   forall (base: ireg) ofs k (rs: regset) v,
-  Mem.loadv chunk m (Val.offset_ptr rs#base ofs) (comp_of fn) = Some v ->
+  Mem.loadv chunk m (Val.offset_ptr rs#base ofs) (Some (comp_of fn)) = Some v ->
   base <> X31 -> rd <> PC ->
   exists rs',
      exec_straight ge fn (indexed_memory_access mk_instr base ofs k) rs m k rs' m
@@ -1184,7 +1184,7 @@ Qed.
 Lemma loadind_correct:
   forall (base: ireg) ofs ty dst k c (rs: regset) m v,
   loadind base ofs ty dst k = OK c ->
-  Mem.loadv (chunk_of_type ty) m (Val.offset_ptr rs#base ofs) (comp_of fn) = Some v ->
+  Mem.loadv (chunk_of_type ty) m (Val.offset_ptr rs#base ofs) (Some (comp_of fn)) = Some v ->
   base <> X31 ->
   exists rs',
      exec_straight ge fn c rs m k rs' m
@@ -1195,8 +1195,8 @@ Proof.
   assert (A: exists mk_instr,
                 c = indexed_memory_access mk_instr base ofs k
              /\ forall base' ofs' rs',
-                   exec_instr ge fn (mk_instr base' ofs') rs' m =
-                   exec_load ge (chunk_of_type ty) rs' m (preg_of dst) base' ofs').
+                   exec_instr ge fn (mk_instr base' ofs') rs' m (comp_of fn) =
+                   exec_load ge (chunk_of_type ty) rs' m (preg_of dst) base' ofs' (comp_of fn) false).
   { unfold loadind in TR. destruct ty, (preg_of dst); inv TR; econstructor; split; eauto. }
   destruct A as (mk_instr & B & C). subst c. 
   eapply indexed_load_access_correct; eauto with asmgen.
@@ -1224,7 +1224,7 @@ Qed.
 
 Lemma loadind_ptr_correct:
   forall (base: ireg) ofs (dst: ireg) k (rs: regset) m v,
-  Mem.loadv Mptr m (Val.offset_ptr rs#base ofs) (comp_of fn) = Some v ->
+  Mem.loadv Mptr m (Val.offset_ptr rs#base ofs) (Some (comp_of fn)) = Some v ->
   base <> X31 ->
   exists rs',
      exec_straight ge fn (loadind_ptr base ofs dst k) rs m k rs' m
@@ -1271,10 +1271,10 @@ Qed.
 Lemma transl_load_access_correct:
   forall chunk (mk_instr: ireg -> offset -> instruction) addr args k c rd (rs: regset) m v v',
   (forall base ofs rs,
-     exec_instr ge fn (mk_instr base ofs) rs m = exec_load ge chunk rs m rd base ofs) ->
+     exec_instr ge fn (mk_instr base ofs) rs m (comp_of fn) = exec_load ge chunk rs m rd base ofs (comp_of fn) false) ->
   transl_memory_access mk_instr addr args k = OK c ->
   eval_addressing ge rs#SP addr (map rs (map preg_of args)) = Some v ->
-  Mem.loadv chunk m v (comp_of fn) = Some v' ->
+  Mem.loadv chunk m v (Some (comp_of fn)) = Some v' ->
   rd <> PC ->
   exists rs',
      exec_straight ge fn c rs m k rs' m
@@ -1315,7 +1315,7 @@ Lemma transl_load_correct:
   forall chunk addr args dst k c (rs: regset) m a v,
   transl_load chunk addr args dst k = OK c ->
   eval_addressing ge rs#SP addr (map rs (map preg_of args)) = Some a ->
-  Mem.loadv chunk m a (comp_of fn) = Some v ->
+  Mem.loadv chunk m a (Some (comp_of fn)) = Some v ->
   exists rs',
      exec_straight ge fn c rs m k rs' m
   /\ rs'#(preg_of dst) = v
@@ -1325,7 +1325,7 @@ Proof.
   assert (A: exists mk_instr,
       transl_memory_access mk_instr addr args k = OK c
    /\ forall base ofs rs,
-        exec_instr ge fn (mk_instr base ofs) rs m = exec_load ge chunk rs m (preg_of dst) base ofs).
+        exec_instr ge fn (mk_instr base ofs) rs m (comp_of fn) = exec_load ge chunk rs m (preg_of dst) base ofs (comp_of fn) false).
   { unfold transl_load in TR; destruct chunk; ArgsInv; econstructor; (split; [eassumption|auto]). }
   destruct A as (mk_instr & B & C).
   eapply transl_load_access_correct; eauto with asmgen.
@@ -1360,8 +1360,8 @@ Qed.
 
 Lemma make_epilogue_correct:
   forall ge0 f m stk soff cs m' ms rs k tm,
-  load_stack m (Vptr stk soff) Tptr f.(fn_link_ofs) (comp_of f) = Some (parent_sp cs) ->
-  load_stack m (Vptr stk soff) Tptr f.(fn_retaddr_ofs) (comp_of f) = Some (parent_ra cs) ->
+  load_stack m (Vptr stk soff) Tptr f.(fn_link_ofs) (Some (comp_of f)) = Some (parent_sp cs) ->
+  load_stack m (Vptr stk soff) Tptr f.(fn_retaddr_ofs) (Some (comp_of f)) = Some (parent_ra cs) ->
   Mem.free m stk 0 f.(fn_stacksize) (comp_of f) = Some m' ->
   agree ms (Vptr stk soff) rs ->
   Mem.extends m tm ->
